Add Handler instances for Error #119

base/coq/Free/HandlerInstances.v
@@ -1,6 +1,7 @@
 (** Instances for the Handler class. *)
 
 From Base Require Import Free.
+From Base Require Import Free.Instance.Error.
 From Base Require Import Free.Instance.Identity.
 From Base Require Import Free.Instance.Maybe.
 From Base Require Import Free.Instance.ND.
@@ -38,6 +39,27 @@ Instance HandlerMaybe (A B : Type)
   handle p := run (runMaybe (nf p))
 }.
 
+(* Error :+: Identity handler *)
+
+Definition SErrId := Comb.Shape (Error.Shape string) Identity.Shape.
+Definition PErrId := Comb.Pos (@Error.Pos string) Identity.Pos.
+
+Instance HandlerError (A B : Type)
+  `{Normalform SErrId PErrId A B} :
+ Handler SErrId PErrId A (B + string) := {
+  handle p := run (runError (nf p))
+}.
+
+Definition pUndefined {Shape : Type} {Pos : Shape -> Type} (P : Partial Shape Pos)
+  := @undefined Shape Pos P (Bool Shape Pos).
+Definition pError {Shape : Type} {Pos : Shape -> Type} (P : Partial Shape Pos) (msg : string)
+  := @error Shape Pos P (Bool Shape Pos) msg.
+
+Compute handle (pUndefined (Maybe.Partial _ _)).
+Compute handle (pUndefined (Error.Partial _ _)).
+Compute handle (pError (Maybe.Partial _ _) "Nope" ).
+Compute handle (pError (Error.Partial _ _) "Nope" ).
+
 (* ND :+: Identity handler *)
 Definition SNDId := Comb.Shape ND.Shape Identity.Shape.
 Definition PNDId := Comb.Pos ND.Pos Identity.Pos.
@@ -71,6 +93,10 @@ Instance HandlerShare (A B : Type)
 }.
 
 (* Two effects *)
+
+(* NOTE: There is no handler for an effect stack that contains both the Error and
+   Maybe effects. Both effects model partiality, but only one interpretation of
+   partiality is used at a time. *)
 
 (* Share :+: ND :+: Identity handler *)
 
@@ -107,6 +133,9 @@ Instance HandlerMaybeShare (A B : Type)
 }.
 
 (* Maybe :+: ND :+: Identity handler *)
+(* If an undefined value is evaluated in one non-deterministic branch of a program,
+   it should not affect the other branches.
+   Therefore, the maybe effect is handled before the non-determinism effect. *)
 
 Definition SMaybeND := Comb.Shape Maybe.Shape (Comb.Shape ND.Shape Identity.Shape).
 Definition PMaybeND := Comb.Pos Maybe.Pos (Comb.Pos ND.Pos Identity.Pos).
@@ -118,6 +147,9 @@ Instance HandlerMaybeND (A B : Type)
 }.
 
 (* Maybe :+: Trace :+: Identity handler *)
+(* In Haskell, when an undefined value is evaluated in a traced program, 
+   the message log until that point is still displayed.
+   Therefore, the maybe effect is handled before the tracing effect. *)
 
 Definition SMaybeTrc := Comb.Shape Maybe.Shape (Comb.Shape Trace.Shape Identity.Shape).
 Definition PMaybeTrc := Comb.Pos Maybe.Pos (Comb.Pos Trace.Pos Identity.Pos).
@@ -128,12 +160,46 @@ Instance HandlerMaybeTrc (A B : Type)
   handle p := collectMessages (run (runTracing (runMaybe (nf p))))
 }.
 
+(* Error :+: Share :+: Identity handler *)
 
-(*
-Instance HandlerTraceMaybe
+Definition SErrShr := Comb.Shape (Error.Shape string) (Comb.Shape Share.Shape Identity.Shape).
+Definition PErrShr := Comb.Pos (@Error.Pos string) (Comb.Pos Share.Pos Identity.Pos).
 
-Instance Handler NDMaybe.
-*)
+Instance HandlerErrorShare (A B : Type)
+                               `{Normalform SErrShr PErrShr A B} :
+ Handler SErrShr PErrShr A (B + string) := {
+  handle p := run (runEmptySharing (0,0) (runError (nf p)))
+}.
+
+(* Error :+: ND :+: Identity handler *)
+(* If an error is thrown in one non-deterministic branch of a program,
+   it should not affect the other branches.
+   Therefore, the error effect is handled before the non-determinism effect. *)
+
+Definition SErrND := Comb.Shape (Error.Shape string) (Comb.Shape ND.Shape Identity.Shape).
+Definition PErrND := Comb.Pos (@Error.Pos string) (Comb.Pos ND.Pos Identity.Pos).
+
+Instance HandlerErrorND (A B : Type)
+                               `{Normalform SErrND PErrND A B} :
+ Handler SErrND PErrND A (list (B + string)) := {
+  handle p := collectVals (run (runChoice (runError (nf p))))
+}.
+
+(* Error :+: Trace :+: Identity handler *)
+(* In Haskell, when an error is thrown in a traced program, the message log until that point
+   is displayed alongside the error message.
+   Therefore, the error effect is handled before the tracing effect. *)
+
+Definition SErrorTrc := Comb.Shape (Error.Shape string) (Comb.Shape Trace.Shape Identity.Shape).
+Definition PErrorTrc := Comb.Pos (@Error.Pos string) (Comb.Pos Trace.Pos Identity.Pos).
+
+Instance HandlerErrorTrc (A B : Type)
+                               `{Normalform SErrorTrc PErrorTrc A B} :
+ Handler SErrorTrc PErrorTrc A ((B + string) * list string) := {
+  handle p := collectMessages (run (runTracing (runError (nf p))))
+}.
+
+Compute handle (trace "Hey!" (trace "Ho!" (error "Nope"))).
 
 (* Trace :+: ND :+: Identity handler *)
 
@@ -209,4 +275,60 @@ Instance HandlerMaybeTrcND (A B : Type)
   handle p := map (@collectMessages (option B))
                   (@collectVals (option B * list (option Sharing.ID * string))
                                 (run (runChoice (runTracing (runMaybe (nf p))))))
+}.
+
+(* Error :+: Share :+: ND :+: Identity handler *)
+
+Definition SErrShrND :=
+  Comb.Shape (Error.Shape string)
+    (Comb.Shape Share.Shape
+      (Comb.Shape ND.Shape Identity.Shape)).
+
+Definition PErrShrND :=
+  Comb.Pos (@Error.Pos string)
+    (Comb.Pos Share.Pos
+      (Comb.Pos ND.Pos Identity.Pos)).
+
+Instance HandlerErrorSharingND (A B : Type)
+                               `{Normalform SErrShrND PErrShrND A B} :
+ Handler SErrShrND PErrShrND A (list (B + string)) := {
+  handle p := collectVals (run (runChoice (runNDSharing (0,0) (runError (nf p)))))
+}.
+
+(* Error :+: Share :+: Trace :+: Identity handler *)
+
+Definition SErrShrTrc :=
+  Comb.Shape (Error.Shape string)
+    (Comb.Shape Share.Shape
+      (Comb.Shape Trace.Shape Identity.Shape)).
+
+Definition PErrShrTrc :=
+  Comb.Pos (@Error.Pos string)
+    (Comb.Pos Share.Pos
+      (Comb.Pos Trace.Pos Identity.Pos)).
+
+Instance HandlerErrorShareTrace (A B : Type)
+                               `{Normalform SErrShrTrc PErrShrTrc A B} :
+ Handler SErrShrTrc PErrShrTrc A ((B + string) * list string) := {
+  handle p := collectMessages (run (runTracing (runTraceSharing (0,0) (runError (nf p)))))
+}.
+
+(* Error :+: Trace :+: ND :+: Identity handler *)
+
+Definition SErrTrcND :=
+  Comb.Shape (Error.Shape string)
+    (Comb.Shape Trace.Shape
+      (Comb.Shape ND.Shape Identity.Shape)).
+
+Definition PErrTrcND :=
+  Comb.Pos (@Error.Pos string)
+    (Comb.Pos Trace.Pos
+      (Comb.Pos ND.Pos Identity.Pos)).
+
+Instance HandlerErrorTrcND (A B : Type)
+                               `{Normalform SErrTrcND PErrTrcND A B} :
+ Handler SErrTrcND PErrTrcND A (list ((B + string) * list string)) := {
+  handle p := map (@collectMessages (B + string))
+                  (@collectVals ((B + string) * list (option Sharing.ID * string))
+                                (run (runChoice (runTracing (runError (nf p))))))
 }.
